Finish adding comments

src/verification/semantics/skip_contract.lean
@@ -1,8 +1,22 @@
 import verification.semantics.skip_stream
 
+/-!
+# Contraction of indexed streams
+
+In this file, we define the contraction of indexed streams `Stream.contract`.
+This replaces the indexing axis with `() : Unit`, implicitly summing over the
+values of the stream.
+
+## Main results
+  - `contract_eval`: Correctness for `contract`; evaluating `contract s` results in
+    the sum of the values of `s`
+  - `is_lawful (Stream.contract s)`: `s.contract` is lawful assuming `s` is
+
+-/
+
 variables {ι : Type} {α : Type*}
 
-@[simps] def contract (s : Stream ι α) : Stream unit α :=
+@[simps] def Stream.contract (s : Stream ι α) : Stream unit α :=
 { σ := s.σ,
   valid := s.valid,
   ready := s.ready,
@@ -14,15 +28,15 @@ variables [linear_order ι]
 
 section index_lemmas
 
-instance (s : Stream ι α) [is_bounded s] : is_bounded (contract s) :=
+instance (s : Stream ι α) [is_bounded s] : is_bounded (Stream.contract s) :=
 ⟨⟨s.wf_rel, s.wf, λ q hq, begin
   rintro ⟨⟨⟩, b⟩,
-  simp only [contract_skip],
+  simp only [Stream.contract_skip],
   refine (s.wf_valid q hq (s.index q hq, b)).imp_right (and.imp_left _),
   simp [Stream.to_order], exact id,
 end⟩⟩
 
-@[simp] lemma contract_next (s : Stream ι α) (q : s.σ) : (contract s).next q = s.next q := rfl
+@[simp] lemma contract_next (s : Stream ι α) (q : s.σ) : (Stream.contract s).next q = s.next q := rfl
 
 end index_lemmas
 
@@ -30,28 +44,28 @@ section value_lemmas
 variables [add_comm_monoid α]
 
 lemma contract_eval₀ (s : Stream ι α) (q : s.σ) (hq : s.valid q) :
-  (contract s).eval₀ q hq () = finsupp.sum_range (s.eval₀ q hq) :=
+  (Stream.contract s).eval₀ q hq () = finsupp.sum_range (s.eval₀ q hq) :=
 by { simp only [Stream.eval₀], dsimp, split_ifs with hr; simp, }
 
 lemma contract_eval (s : Stream ι α) [is_bounded s] [add_comm_monoid α] (q : s.σ) :
-  (contract s).eval q () = finsupp.sum_range (s.eval q) :=
+  (Stream.contract s).eval q () = finsupp.sum_range (s.eval q) :=
 begin
-  refine @well_founded.induction _ (contract s).wf_rel (contract s).wf _ q _,
+  refine @well_founded.induction _ (Stream.contract s).wf_rel (Stream.contract s).wf _ q _,
   clear q, intros q ih,
   by_cases hq : s.valid q, swap, { simp [hq], },
-  simp only [s.eval_valid _ hq, (contract s).eval_valid _ hq, finsupp.coe_add, pi.add_apply,
-    map_add, ih _ ((contract s).next_wf q hq)], rw [contract_next, contract_eval₀],
+  simp only [s.eval_valid _ hq, (Stream.contract s).eval_valid _ hq, finsupp.coe_add, pi.add_apply,
+    map_add, ih _ ((Stream.contract s).next_wf q hq)], rw [contract_next, contract_eval₀],
 end
 
-lemma contract_mono (s : Stream ι α) : (contract s).is_monotonic :=
-λ q hq i, by { rw [Stream.index'_val hq, punit_eq_star ((contract s).index q hq)], exact bot_le, }
+lemma contract_mono (s : Stream ι α) : (Stream.contract s).is_monotonic :=
+λ q hq i, by { rw [Stream.index'_val hq, punit_eq_star ((Stream.contract s).index q hq)], exact bot_le, }
 
-instance (s : Stream ι α) [is_lawful s] : is_lawful (contract s) :=
+instance (s : Stream ι α) [is_lawful s] : is_lawful (Stream.contract s) :=
 { mono := contract_mono s,
   skip_spec := λ q hq i j hj, begin
     cases j,
     obtain rfl : i = ((), ff) := le_bot_iff.mp hj,
-    simp only [contract_skip, contract_eval, Stream.eval_skip_eq_of_ff],
+    simp only [Stream.contract_skip, contract_eval, Stream.eval_skip_eq_of_ff],
   end }
 
 end value_lemmas
